theories/iSL/Simp.v
@@ -529,7 +529,7 @@ Qed.
 
 Require Import ISL.InvPropQuantifiers.
 
-Definition E_simplified (p: variable) (ψ: form) := simp_form (E p ([ψ],  ⊥)).
+Definition E_simplified (p: variable) (ψ: form) := simp_form (E p [ψ]).
 Definition A_simplified (p: variable) (ψ: form) := simp_form (Af p (ψ)).
 
 (*
